Automation.v
@@ -1,0 +1,6 @@
+Ltac deex :=
+  match goal with
+  | [ H: exists (varname:_), _ |- _ ] =>
+    let name := fresh varname in
+    destruct H as [name ?]
+  end.
