PFun.v
@@ -1,0 +1,69 @@
+Set Implicit Arguments.
+
+Require Import FunctionalExtensionality.
+
+Definition EqDec A := forall (x y:A), {x=y}+{x<>y}.
+Existing Class EqDec.
+
+Definition pfun A V := A -> option V.
+
+Definition upd A {AEQ: EqDec A} V (m: pfun A V) a v : pfun A V :=
+  fun a' => if AEQ a a' then Some v else m a'.
+
+Ltac destruct_match :=
+  match goal with
+  | [ H: context[match ?d with | _ => _ end] |- _ ] =>
+    let Heq := fresh in
+    destruct d eqn:Heq; simpl in H; subst; try congruence
+  | [ |- context[match ?d with | _ => _ end] ] =>
+    let Heq := fresh in
+    destruct d eqn:Heq; simpl; subst; try congruence
+  end.
+
+Theorem upd_eq : forall A {AEQ: EqDec A} V (m: pfun A V) a v,
+    upd m a v a = Some v.
+Proof.
+  unfold upd; intros.
+  destruct_match; auto.
+Qed.
+
+Theorem upd_neq : forall A {AEQ: EqDec A} V (m: pfun A V) a v a',
+    a <> a' ->
+    upd m a v a' = m a'.
+Proof.
+  unfold upd; intros.
+  destruct_match; auto.
+Qed.
+
+Hint Rewrite upd_eq  : upd.
+Hint Rewrite upd_neq using (solve [ auto ]) : upd.
+
+Definition remove A {AEQ: EqDec A} V (m: pfun A V) a : pfun A V :=
+  fun a' => if AEQ a a' then None else m a'.
+
+Lemma remove_eq : forall A {AEQ: EqDec A} V (m: pfun A V) a,
+    remove m a a = None.
+Proof.
+  unfold remove; intros.
+  destruct_match; auto.
+Qed.
+
+Lemma remove_neq : forall A {AEQ: EqDec A} V (m: pfun A V) a a',
+    a <> a' ->
+    remove m a a' = m a'.
+Proof.
+  unfold remove; intros.
+  destruct_match; auto.
+Qed.
+
+Hint Rewrite remove_eq : upd.
+Hint Rewrite remove_neq using (solve [ auto ]) : upd.
+
+Theorem remove_upd : forall A {AEQ:EqDec A} V (m: pfun A V) a v,
+    m a = Some v ->
+    m = upd (remove m a) a v.
+Proof.
+  intros.
+  extensionality a'.
+  destruct (AEQ a a'); subst; autorewrite with upd; auto.
+Qed.
