Makefile
@@ -1,9 +1,12 @@
-SOURCE := Prog.v Threads.v
+SOURCE := PFun.v Prog.v Automation.v Threads.v
 
 VO_FILES := $(SOURCE:.v=.vo)
 
 all: $(VO_FILES)
 
+Prog.vo: PFun.vo
+
+Threads.vo: Prog.vo Automation.vo
 
 %.vo: %.v
 	coqc $<
